Outline Proof Correctness Message Body (#237)
* Outline Proof Correctness Message Body

Includes all requirements, expected function definitions. Avoids arithmetic problems in EncryptMessageBody method

* Finished the proofs of encryption methods

* Small refactoring

* Small refactoring and removed export

Export does not support exporting predicates from datatypes. This will cause errors if the methods are called outside of the module.

* Initial Work Deserialize

* Work in progress on MessageBody

feat: Added draft of postconditions DecryptFrame

* Work in progress messagebody

* Added proof Decrypt Frame

fix: Finished the proof of DecryptFrame method

* Finished Encrypt MessageBody

feat: Proved all post conditions of MessageBody

* Set stream file to the needed file which is not merged yet

* Update MessageBody.dfy

feat: Small strengtening encrypt post conditions

* Moved facts from Encryption to AESEncrypt

fix: Moved EncryptMock and DecryptMock yo AESEncryption

* Added export provides back

fix:Added export back

* Fix: Changed predicates to match pattern external

* fix: Added export back

* Added changes rustan bugfix precondition

fix: Removed incorrect pre condition

* Updated dafny version

fix: updated dafny version to use new features

* Fixed problem verfification AESKeyring

fix: Keyring called outdated method not containing required post condition

* Added missing failure check removed unused lemmas

Chore: Removed unused lemmas
Fix: Added failure check if final frame is too big in decrypt

* Speedup and removed subsequence to frames

chore: Created speed up by removing unwanted definitions

* Fix updated buildspec

* Update MessageBody.dfy

* Made changes based on review

* Added prerambe comment

chore: Added comment to messageBody giving a rough outline of the specs

* Bugfixes

* Bugfix changes cs file to match names

* Updated MessageBody based on PR feedback

chore: Added extra comments
chore: General refactoring

* Revert "Updated MessageBody based on PR feedback"

This reverts commit 5b3959b1ca1e51a43e03466725cf37814f446795.

* Updates based on comments

Chore: Updated comments and removed unwanted commit
Chore: Changed sloppy error message removed unwanted file changes

* Removed expect statements

* Simple reformatting changes

Co-authored-by: wouter <wouter@amazon.com>

src/SDK/MessageBody.dfy
@@ -10,10 +10,11 @@ include "../Util/UTF8.dfy"
 
 module MessageBody {
   export
-    provides EncryptMessageBody
-    provides DecryptFramedMessageBody, DecryptNonFramedMessageBody
-    provides StandardLibrary, UInt, Msg, AlgorithmSuite, Materials, Streams
-
+    provides EncryptMessageBody, DecryptFramedMessageBody, DecryptNonFramedMessageBody,
+      StandardLibrary, UInt, Msg, AlgorithmSuite, Materials, Streams, FramesToSequence, 
+      FrameToSequence, ValidFrames, FramesEncryptPlaintext
+    reveals Frame, Frame.Valid
+    
   import opened StandardLibrary
   import opened UInt = StandardLibrary.UInt
   import AlgorithmSuite
@@ -24,7 +25,32 @@ module MessageBody {
   import EncryptionSuites
   import UTF8
 
-  datatype BodyAADContent = RegularFrame | FinalFrame | SingleBlock
+  datatype BodyAADContent = AADRegularFrame | AADFinalFrame | AADSingleBlock
+
+  /**
+    The behavior of the methods in this file are specified in https://github.com/awslabs/aws-encryption-sdk-specification/blob/master/data-format/message-body.md
+    The Frame datatype has been introduced in the validation of this file. This datatype is only used for the validation. 
+    The methods in this file serialize and deserialize some plaintext to frames. Frame are encoded in a sequence of bytes.
+  */
+
+  // Predicate all conditions which should hold for any valid sequence of frames 
+  predicate ValidFrames(frames: seq<Frame>) {
+    0 < |frames| < UINT32_LIMIT &&
+    forall i | 0 <= i < |frames| ::
+      var frame := frames[i];
+      frame.Valid() &&
+      (if i == |frames| - 1 then frame.FinalFrame? else frame.RegularFrame?) &&
+      frame.seqNum as int == i + START_SEQUENCE_NUMBER as int &&
+      (forall j | i < j < |frames| :: frame.iv != frames[j].iv)
+  }
+
+  datatype Frame = RegularFrame(seqNum: uint32, iv: seq<uint8>, encContent: seq<uint8>, authTag: seq<uint8>) |
+                   FinalFrame(seqNum: uint32, iv: seq<uint8>, encContent: seq<uint8>, authTag: seq<uint8>)
+  {
+    predicate Valid() {
+      |encContent| < UINT32_LIMIT
+    }
+  }
 
   const BODY_AAD_CONTENT_REGULAR_FRAME: string := "AWSKMSEncryptionClient Frame"
   const BODY_AAD_CONTENT_FINAL_FRAME: string := "AWSKMSEncryptionClient Final Frame"
@@ -32,150 +58,454 @@ module MessageBody {
 
   function method BodyAADContentTypeString(bc: BodyAADContent): string {
     match bc
-    case RegularFrame => BODY_AAD_CONTENT_REGULAR_FRAME
-    case FinalFrame => BODY_AAD_CONTENT_FINAL_FRAME
-    case SingleBlock => BODY_AAD_CONTENT_SINGLE_BLOCK
+    case AADRegularFrame => BODY_AAD_CONTENT_REGULAR_FRAME
+    case AADFinalFrame => BODY_AAD_CONTENT_FINAL_FRAME
+    case AADSingleBlock => BODY_AAD_CONTENT_SINGLE_BLOCK
   }
 
   const START_SEQUENCE_NUMBER: uint32 := 1
   const ENDFRAME_SEQUENCE_NUMBER: uint32 := 0xFFFF_FFFF
   const NONFRAMED_SEQUENCE_NUMBER: uint32 := 1
 
-  method EncryptMessageBody(plaintext: seq<uint8>, frameLength: int, messageID: Msg.MessageID, key: seq<uint8>, algorithmSuiteID: AlgorithmSuite.ID) returns (res: Result<seq<uint8>>)
+  function method IVSeq(algorithmSuiteID: AlgorithmSuite.ID, sequenceNumber: uint32): seq<uint8> {
+    seq(algorithmSuiteID.IVLength() - 4, _ => 0) + UInt32ToSeq(sequenceNumber)
+  }
+
+  lemma IVSeqDistinct(algorithmSuiteID: AlgorithmSuite.ID, m: uint32, n: uint32)
+    requires m != n
+    ensures IVSeq(algorithmSuiteID, m) != IVSeq(algorithmSuiteID, n)
+  {
+    var paddingLength := algorithmSuiteID.IVLength() - 4;
+    assert IVSeq(algorithmSuiteID, m)[paddingLength..] == UInt32ToSeq(m);
+    assert IVSeq(algorithmSuiteID, n)[paddingLength..] == UInt32ToSeq(n);
+    UInt32SeqSerializeDeserialize(m);
+    UInt32SeqSerializeDeserialize(n);
+  }
+
+  // Converts sequence of Frames to a sequence encoding all frames
+  function FramesToSequence(frames : seq<Frame>): seq<uint8>
+    requires |frames| < UINT32_LIMIT
+    requires forall frame | frame in frames :: frame.Valid()
+  {
+    if frames == [] then
+      []
+    else
+      FramesToSequence(frames[..|frames| - 1]) + FrameToSequence(frames[|frames| - 1])
+  }
+
+  lemma ExtendFramesToSequence(frames: seq<Frame>, frame: Frame)
+    requires |frames| < UINT32_LIMIT - 1
+    requires forall frame | frame in frames :: frame.Valid()
+    requires frame.Valid()
+    ensures FramesToSequence(frames + [frame]) == FramesToSequence(frames) + FrameToSequence(frame)
+  {
+  }
+
+  // Converts Frame to a sequence encoding a frame
+  function FrameToSequence(frame: Frame): (res: seq<uint8>)
+    requires frame.Valid()
+    ensures match frame
+      case RegularFrame(_, iv: seq<uint8>, encContent: seq<uint8>, authTag: seq<uint8>) =>
+        4 + |iv| + |encContent| + |authTag| == |res|
+      case FinalFrame(seqNum: uint32, iv: seq<uint8>, encContent: seq<uint8>, authTag: seq<uint8>) =>
+        4 + 4 + |iv| + 4 + |encContent| + |authTag| == |res|
+  {
+    match frame 
+      case RegularFrame(seqNum, iv, encContent, authTag) =>
+        var seqNumSeq := UInt32ToSeq(seqNum);
+        seqNumSeq + iv + encContent + authTag
+      case FinalFrame(seqNum, iv, encContent, authTag) =>
+        var seqNumEndSeq := UInt32ToSeq(ENDFRAME_SEQUENCE_NUMBER);
+        var seqNumSeq := UInt32ToSeq(seqNum);
+        var encContentLengthSeq := UInt32ToSeq(|encContent| as uint32);
+        seqNumEndSeq + seqNumSeq + iv + encContentLengthSeq + encContent + authTag
+  }
+
+  /**
+    Predicate states that frames encrypt plaintext
+    
+      Plaintext is split into chunks of frameLength. One chunck is encrypted in one frame. Reasoning about chunks makes proving predicate easier 
+        FramesEncryptPlaintextSegments: States that sequence of frames decrypts to sequence of chunks
+        SumPlaintextSegments: States that sum of chunks is the plaintext
+   */
+  predicate FramesEncryptPlaintext(frames: seq<Frame>, plaintext: seq<uint8>)
+  {
+    exists plaintextSeg: seq<seq<uint8>> ::
+      FramesEncryptPlaintextSegments(frames, plaintextSeg) && SumPlaintextSegments(plaintextSeg) == plaintext
+  }
+
+  predicate FramesEncryptPlaintextSegments(frames: seq<Frame>, plaintextSeg: seq<seq<uint8>>)
+  {
+    if |frames| != |plaintextSeg| then 
+      false
+    else
+      if frames == [] then
+        true
+      else
+        FramesEncryptPlaintextSegments(frames[..|frames| - 1], plaintextSeg[..|frames| - 1]) &&
+        AESEncryption.CiphertextGeneratedWithPlaintext(frames[|frames| - 1].encContent, plaintextSeg[|frames| - 1])
+  }
+
+  // Steps for inductive proofs EncryptMessageBody  
+  lemma ExtendFramesEncryptPlaintextSegments(frames: seq<Frame>, plaintextSeg: seq<seq<uint8>>, frame: Frame, plaintextFrame: seq<uint8>)
+    requires FramesEncryptPlaintextSegments(frames, plaintextSeg)
+    requires AESEncryption.CiphertextGeneratedWithPlaintext(frame.encContent, plaintextFrame)
+    ensures FramesEncryptPlaintextSegments(frames + [frame], plaintextSeg + [plaintextFrame])
+  {
+  }
+
+  function SumPlaintextSegments(plaintextSeg: seq<seq<uint8>>): seq<uint8>
+  {
+    if plaintextSeg == [] then
+      []
+    else
+      SumPlaintextSegments(plaintextSeg[..|plaintextSeg| - 1]) + plaintextSeg[|plaintextSeg| - 1]
+  }
+
+  lemma ExtendSumPlaintextSegments(plaintextSeg: seq<seq<uint8>>, plaintextFrame: seq<uint8>)
+    ensures SumPlaintextSegments(plaintextSeg + [plaintextFrame]) == SumPlaintextSegments(plaintextSeg) + plaintextFrame
+  {
+  }
+
+  method EncryptMessageBody(plaintext: seq<uint8>, frameLength: int, messageID: Msg.MessageID, key: seq<uint8>, algorithmSuiteID: AlgorithmSuite.ID)
+      returns (result: Result<seq<uint8>>)
     requires |key| == algorithmSuiteID.KeyLength()
     requires 0 < frameLength < UINT32_LIMIT
-  {
+    ensures match result
+      case Failure(e) => true
+      case Success(resultSuccess) => exists frames: seq<Frame> | ValidFrames(frames) ::
+        && FramesToSequence(frames) == resultSuccess
+        && FramesEncryptPlaintext(frames, plaintext)
+  { 
     var body := [];
-    var n, sequenceNumber := 0, START_SEQUENCE_NUMBER;
+    var n : int, sequenceNumber := 0, START_SEQUENCE_NUMBER;
+    ghost var frames : seq<Frame> := [];
+    ghost var plaintextSeg := [];
+    
     while n + frameLength < |plaintext|
-      invariant 0 <= n <= |plaintext|
+      invariant |plaintext| != 0 ==> 0 <= n < |plaintext|
+      invariant |plaintext| == 0 ==> 0 == n
       invariant START_SEQUENCE_NUMBER <= sequenceNumber <= ENDFRAME_SEQUENCE_NUMBER
+      invariant |frames| == (sequenceNumber - START_SEQUENCE_NUMBER) as int
+      invariant forall i | 0 <= i < |frames| :: // Sequence of frames is valid
+        var frame := frames[i];
+        frame.Valid() &&
+        frame.RegularFrame? &&
+        frame.seqNum as int == i + START_SEQUENCE_NUMBER as int
+      invariant forall i | 0 <= i < |frames| :: frames[i].iv == IVSeq(algorithmSuiteID, frames[i].seqNum)
+      invariant FramesToSequence(frames) == body
+      invariant FramesEncryptPlaintextSegments(frames, plaintextSeg) // Frames decrypt to chunks of plaintext
+      invariant SumPlaintextSegments(plaintextSeg) == plaintext[..n] // Chunks of plaintext sum up to plaintexts
     {
       if sequenceNumber == ENDFRAME_SEQUENCE_NUMBER {
         return Failure("too many frames");
       }
       var plaintextFrame := plaintext[n..n + frameLength];
-      var regularFrame :- EncryptRegularFrame(algorithmSuiteID, key, frameLength, messageID, plaintextFrame, sequenceNumber);
-      body := body + regularFrame;
+      var regularFrame, frame := EncryptRegularFrame(algorithmSuiteID, key, frameLength, messageID, plaintextFrame, sequenceNumber);
+      if regularFrame.IsFailure() {
+        return regularFrame.PropagateFailure();
+      }
+      assert frame.iv == IVSeq(algorithmSuiteID, sequenceNumber);
+
+      // Proofs that invariant holds after loop
+      ExtendFramesToSequence(frames, frame); 
+      ExtendFramesEncryptPlaintextSegments(frames, plaintextSeg, frame, plaintextFrame);
+      ExtendSumPlaintextSegments(plaintextSeg, plaintextFrame);
+      frames := frames + [frame];
+      body := body + regularFrame.Extract();
+      plaintextSeg := plaintextSeg + [plaintextFrame];
+      
       n, sequenceNumber := n + frameLength, sequenceNumber + 1;
+      assert SumPlaintextSegments(plaintextSeg) == plaintext[..n];
     }
-    var finalFrame :- EncryptFinalFrame(algorithmSuiteID, key, frameLength, messageID, plaintext[n..], sequenceNumber);
-    body := body + finalFrame;
-    return Success(body);
+
+    var finalFrameResult, finalFrame := EncryptFinalFrame(algorithmSuiteID, key, frameLength, messageID, plaintext[n..], sequenceNumber);
+    if finalFrameResult.IsFailure() {
+      return finalFrameResult.PropagateFailure();
+    }
+    var finalFrameSequence := finalFrameResult.Extract();
+    assert finalFrame.iv == IVSeq(algorithmSuiteID, sequenceNumber);
+    ExtendFramesToSequence(frames, finalFrame);
+    ExtendFramesEncryptPlaintextSegments(frames, plaintextSeg, finalFrame, plaintext[n..]);
+    ExtendSumPlaintextSegments(plaintextSeg, plaintext[n..]);
+    frames := frames + [finalFrame];
+    body := body + finalFrameSequence;
+    plaintextSeg := plaintextSeg + [plaintext[n..]];
+    assert ValidFrames(frames) by {
+      forall i,j | 0 <= i < j < |frames|
+        ensures frames[i].iv != frames[j].iv
+      {
+        assert frames[i].seqNum as int == i + START_SEQUENCE_NUMBER as int;
+        assert frames[j].seqNum as int == j + START_SEQUENCE_NUMBER as int;
+        assert frames[i].iv == IVSeq(algorithmSuiteID, frames[i].seqNum);
+        assert frames[j].iv == IVSeq(algorithmSuiteID, frames[j].seqNum);
+        IVSeqDistinct(algorithmSuiteID, frames[i].seqNum, frames[j].seqNum);
+      }
+    }
+
+    result := Success(body);
   }
 
   method EncryptRegularFrame(algorithmSuiteID: AlgorithmSuite.ID, key: seq<uint8>, ghost frameLength: int,
                              messageID: Msg.MessageID, plaintext: seq<uint8>, sequenceNumber: uint32)
-      returns (res: Result<seq<uint8>>)
+      returns (res: Result<seq<uint8>>, ghost regFrame: Frame)
     requires |key| == algorithmSuiteID.KeyLength()
-    requires 0 < frameLength && START_SEQUENCE_NUMBER <= sequenceNumber <= ENDFRAME_SEQUENCE_NUMBER
+    requires 0 < frameLength < UINT32_LIMIT && START_SEQUENCE_NUMBER <= sequenceNumber <= ENDFRAME_SEQUENCE_NUMBER
     requires |plaintext| < UINT32_LIMIT
     requires |plaintext| == frameLength && sequenceNumber != ENDFRAME_SEQUENCE_NUMBER
     requires 4 <= algorithmSuiteID.IVLength()
+    ensures match res 
+      case Failure(e) => true
+      case Success(resultSuccess) => 
+           // Decrypt serialized frame back to frame and state that it is equal to the ghost frame
+        4 + algorithmSuiteID.IVLength() + algorithmSuiteID.TagLength() + frameLength == |resultSuccess|
+        && var iv := IVSeq(algorithmSuiteID, sequenceNumber);
+        var encContent := resultSuccess[4 + algorithmSuiteID.IVLength()..4 + algorithmSuiteID.IVLength() + frameLength];
+        var authTag := resultSuccess[4 + algorithmSuiteID.IVLength() + frameLength..];
+        var frame := RegularFrame(sequenceNumber, iv, encContent, authTag);
+        frame == regFrame
+        && FrameToSequence(regFrame) == resultSuccess
+        && AESEncryption.CiphertextGeneratedWithPlaintext(frame.encContent, plaintext)
   {
     var seqNumSeq := UInt32ToSeq(sequenceNumber);
     var unauthenticatedFrame := seqNumSeq;
+    var iv := IVSeq(algorithmSuiteID, sequenceNumber);
+    var aad := BodyAAD(messageID, AADRegularFrame, sequenceNumber, |plaintext| as uint64);
+    
+    var encryptionOutputResult := AESEncryption.AESEncrypt(algorithmSuiteID.EncryptionSuite(), iv, key, plaintext, aad);
+    if encryptionOutputResult.IsFailure() {
+      res := encryptionOutputResult.PropagateFailure();
+      return;
+    }
+    var encryptionOutput := encryptionOutputResult.Extract();
+    ghost var frame := RegularFrame(sequenceNumber, iv, encryptionOutput.cipherText, encryptionOutput.authTag);
 
-    var iv := seq(algorithmSuiteID.IVLength() - 4, _ => 0) + UInt32ToSeq(sequenceNumber);
     SeqWithUInt32Suffix(iv, sequenceNumber as nat);  // this proves SeqToNat(iv) == sequenceNumber as nat
     unauthenticatedFrame := unauthenticatedFrame + iv;
-
-    var aad := BodyAAD(messageID, RegularFrame, sequenceNumber, |plaintext| as uint64);
-
-    var encryptionOutput :- AESEncryption.AESEncrypt(algorithmSuiteID.EncryptionSuite(), iv, key, plaintext, aad);
     unauthenticatedFrame := unauthenticatedFrame + encryptionOutput.cipherText + encryptionOutput.authTag;
 
-    return Success(unauthenticatedFrame);
+    return Success(unauthenticatedFrame), frame;
   }
 
-  method EncryptFinalFrame(algorithmSuiteID: AlgorithmSuite.ID, key: seq<uint8>, frameLength: int,
+  method EncryptFinalFrame(algorithmSuiteID: AlgorithmSuite.ID, key: seq<uint8>, frameLength: int, 
                            messageID: Msg.MessageID, plaintext: seq<uint8>, sequenceNumber: uint32)
-      returns (res: Result<seq<uint8>>)
+      returns (res: Result<seq<uint8>>, ghost finalFrame: Frame)
     requires |key| == algorithmSuiteID.KeyLength()
-    requires 0 < frameLength && START_SEQUENCE_NUMBER <= sequenceNumber <= ENDFRAME_SEQUENCE_NUMBER
-    requires |plaintext| < UINT32_LIMIT
+    requires START_SEQUENCE_NUMBER <= sequenceNumber <= ENDFRAME_SEQUENCE_NUMBER
+    requires 0 <= |plaintext| < UINT32_LIMIT
+    requires 0 < frameLength < UINT32_LIMIT
     requires |plaintext| <= frameLength
     requires 4 <= algorithmSuiteID.IVLength()
+    ensures match res 
+      case Failure(e) => true
+      case Success(resultSuccess) => 
+        // Decrypt serialized frame back to frame and state that it is equal to the ghost frame
+        4 + 4 + algorithmSuiteID.IVLength() + 4 + algorithmSuiteID.TagLength() <= |resultSuccess| 
+          <= 4 + 4 + algorithmSuiteID.IVLength() + 4 + algorithmSuiteID.TagLength() + frameLength
+        && var contentLength : uint32 := SeqToUInt32(resultSuccess[4+4+algorithmSuiteID.IVLength()..4+4+algorithmSuiteID.IVLength()+4]);
+        |resultSuccess| == 4 + 4 + algorithmSuiteID.IVLength() + 4 + contentLength as int + algorithmSuiteID.TagLength() 
+        && resultSuccess[..4] == UInt32ToSeq(ENDFRAME_SEQUENCE_NUMBER)
+        && |plaintext| == SeqToUInt32(resultSuccess[4 + 4 + algorithmSuiteID.IVLength()..4 + 4 + algorithmSuiteID.IVLength() + 4]) as int &&
+        var iv := IVSeq(algorithmSuiteID, sequenceNumber);
+        var encContent := resultSuccess[4 + 4 + algorithmSuiteID.IVLength() + 4..][..|plaintext|];
+        var authTag := resultSuccess[4 + 4 + algorithmSuiteID.IVLength() + 4 + |plaintext|..];
+        var frame := FinalFrame(sequenceNumber, iv, encContent, authTag);
+        FrameToSequence(frame) == resultSuccess
+        && finalFrame == frame
+        && AESEncryption.CiphertextGeneratedWithPlaintext(frame.encContent, plaintext)
   {
     var unauthenticatedFrame := UInt32ToSeq(ENDFRAME_SEQUENCE_NUMBER);
     var seqNumSeq := UInt32ToSeq(sequenceNumber);
     unauthenticatedFrame := unauthenticatedFrame + seqNumSeq;
 
-    var iv := seq(algorithmSuiteID.IVLength() - 4, _ => 0) + UInt32ToSeq(sequenceNumber);
+    var iv := IVSeq(algorithmSuiteID, sequenceNumber);
     SeqWithUInt32Suffix(iv, sequenceNumber as nat);  // this proves SeqToNat(iv) == sequenceNumber as nat
     unauthenticatedFrame := unauthenticatedFrame + iv;
-
     unauthenticatedFrame := unauthenticatedFrame + UInt32ToSeq(|plaintext| as uint32);
 
-    var aad := BodyAAD(messageID, FinalFrame, sequenceNumber, |plaintext| as uint64);
+    var aad := BodyAAD(messageID, AADFinalFrame, sequenceNumber, |plaintext| as uint64);
 
-    var encryptionOutput :- AESEncryption.AESEncrypt(algorithmSuiteID.EncryptionSuite(), iv, key, plaintext, aad);
-    unauthenticatedFrame := unauthenticatedFrame + encryptionOutput.cipherText + encryptionOutput.authTag;
-
-    return Success(unauthenticatedFrame);
-  }
-
-  method DecryptFramedMessageBody(rd: Streams.ByteReader, algorithmSuiteID: AlgorithmSuite.ID, key: seq<uint8>, frameLength: int, messageID: Msg.MessageID) returns (res: Result<seq<uint8>>)
-    requires rd.Valid()
-    requires |key| == algorithmSuiteID.KeyLength()
-    requires 0 < frameLength < UINT32_LIMIT
-    modifies rd.reader`pos
-    ensures rd.Valid()
-  {
-    var plaintext := [];
-    var n := 1;
-    while true
-      invariant rd.Valid()
-      decreases ENDFRAME_SEQUENCE_NUMBER - n
-    {
-      var pair :- DecryptFrame(rd, algorithmSuiteID, key, frameLength, messageID, n);
-      var (framePlaintext, final) := pair;
-      plaintext := plaintext + framePlaintext;
-      if final {
-        break;
-      }
-      n := n + 1;
+    var encryptionOutputResult := AESEncryption.AESEncrypt(algorithmSuiteID.EncryptionSuite(), iv, key, plaintext, aad);
+    if encryptionOutputResult.IsFailure() {
+      res := encryptionOutputResult.PropagateFailure();
+      return;
     }
-    return Success(plaintext);
+    var encryptionOutput := encryptionOutputResult.Extract();
+    unauthenticatedFrame := unauthenticatedFrame + encryptionOutput.cipherText + encryptionOutput.authTag;
+    assert |plaintext| == |encryptionOutput.cipherText|;
+
+    ghost var frame := FinalFrame(sequenceNumber, iv, encryptionOutput.cipherText, encryptionOutput.authTag);
+    finalFrame := frame;
+    assert FrameToSequence(frame) == unauthenticatedFrame;
+    // Show which part of the serialized frame map to which frame variable
+    assert |plaintext| == SeqToUInt32(unauthenticatedFrame[4 + 4 + algorithmSuiteID.IVLength()..4 + 4 + algorithmSuiteID.IVLength() + 4]) as int;
+    assert |unauthenticatedFrame| == 4 + 4 + algorithmSuiteID.IVLength() + 4 + |plaintext| + algorithmSuiteID.TagLength();
+    assert unauthenticatedFrame[4 + 4 + algorithmSuiteID.IVLength() + 4..][..|plaintext|] == encryptionOutput.cipherText;
+
+    return Success(unauthenticatedFrame), finalFrame;
   }
 
-  method DecryptFrame(rd: Streams.ByteReader, algorithmSuiteID: AlgorithmSuite.ID, key: seq<uint8>, frameLength: int, messageID: Msg.MessageID,
-                      expectedSequenceNumber: uint32)
-      returns (res: Result<(seq<uint8>, bool)>)
+  method DecryptFramedMessageBody(rd: Streams.ByteReader, algorithmSuiteID: AlgorithmSuite.ID, key: seq<uint8>, frameLength: int, messageID: Msg.MessageID) 
+      returns (res: Result<seq<uint8>>)
     requires rd.Valid()
     requires |key| == algorithmSuiteID.KeyLength()
     requires 0 < frameLength < UINT32_LIMIT
     modifies rd.reader`pos
     ensures rd.Valid()
     ensures match res
-      case Success((plaintext, final)) =>
-        expectedSequenceNumber == ENDFRAME_SEQUENCE_NUMBER ==> final  // but "final" may come up before this
+      case Failure(_) => true
+      case Success(plaintext) => //Exists a sequence of frames which encrypts the plaintext and is serialized in the read section of the stream
+        old(rd.reader.pos) <= rd.reader.pos <= |rd.reader.data| 
+        && exists frames: seq<Frame> | |frames| < UINT32_LIMIT && (forall frame | frame in frames :: frame.Valid()) 
+            && FramesToSequence(frames) == rd.reader.data[old(rd.reader.pos)..rd.reader.pos] :: 
+              FramesEncryptPlaintext(frames, plaintext)
+  {
+    var plaintext := [];
+    var n: uint32 := 1;
+    ghost var frames: seq<Frame> := [];
+    ghost var plaintextSeg: seq<seq<uint8>> := []; // Chuncks of plaintext which are decrypted from the frame
+
+    while true
+      decreases ENDFRAME_SEQUENCE_NUMBER - n
+      invariant rd.Valid()
+      invariant n as int - 1 == |frames|
+      invariant n <= ENDFRAME_SEQUENCE_NUMBER
+      invariant forall frame | frame in frames :: frame.Valid()
+      invariant old(rd.reader.pos) <= rd.reader.pos <= |rd.reader.data|
+      invariant FramesToSequence(frames) == rd.reader.data[old(rd.reader.pos)..rd.reader.pos]
+      invariant rd.Valid()
+      invariant FramesEncryptPlaintextSegments(frames, plaintextSeg) // All decrypted frames decrypt to the list of plaintext chuncks
+      invariant SumPlaintextSegments(plaintextSeg) == plaintext // The current decrypted frame is the sum of all decrypted chuncks 
+    {
+      var frameWithGhostSeq :- DecryptFrame(rd, algorithmSuiteID, key, frameLength, messageID, n);
+      assert |frameWithGhostSeq.ciphertext| < UINT32_LIMIT;
+      var decryptedFrame := frameWithGhostSeq.frame;
+      ghost var ciphertext := frameWithGhostSeq.ciphertext;
+      assert |ciphertext| < UINT32_LIMIT;
+      ghost var encryptedFrame := if decryptedFrame.FinalFrame? then
+        FinalFrame(decryptedFrame.seqNum, decryptedFrame.iv, ciphertext, decryptedFrame.authTag)
+      else
+        RegularFrame(decryptedFrame.seqNum, decryptedFrame.iv, ciphertext, decryptedFrame.authTag);
+      assert encryptedFrame.Valid();
+      frames := frames + [encryptedFrame];
+
+      var (decryptedFramePlaintext, final) := (decryptedFrame.encContent, decryptedFrame.FinalFrame?);
+      
+      plaintext := plaintext + decryptedFramePlaintext;
+      plaintextSeg := plaintextSeg + [decryptedFramePlaintext];
+      if final {
+        assert FramesEncryptPlaintextSegments(frames, plaintextSeg);
+        assert SumPlaintextSegments(plaintextSeg) == plaintext;
+        break;
+      }
+      n := n + 1;
+    }
+    assert |frames| < UINT32_LIMIT ;
+    assert (forall frame | frame in frames :: frame.Valid()) ;
+    assert FramesToSequence(frames) == rd.reader.data[old(rd.reader.pos)..rd.reader.pos]; 
+    return Success(plaintext);
+  }
+
+  datatype FrameWithGhostSeq = FrameWithGhostSeq(frame: Frame, ghost ciphertext: seq<uint8>)
+
+  method DecryptFrame(rd: Streams.ByteReader, algorithmSuiteID: AlgorithmSuite.ID, key: seq<uint8>, frameLength: int, messageID: Msg.MessageID,
+                      expectedSequenceNumber: uint32)
+      returns (res: Result<FrameWithGhostSeq>)
+    requires rd.Valid()
+    requires |key| == algorithmSuiteID.KeyLength()
+    requires 0 < frameLength < UINT32_LIMIT
+    modifies rd.reader`pos
+    ensures rd.Valid()
+    ensures match res // If the expected sequence number is the end frame sequence number then the frame is the final frame. However, the final frame can arrive earlier
+      case Success(frameWithGhostSeq) =>
+        expectedSequenceNumber == ENDFRAME_SEQUENCE_NUMBER ==> frameWithGhostSeq.frame.FinalFrame? 
+      case Failure(_) => true
+    ensures res.Success? ==> |res.value.ciphertext| < UINT32_LIMIT
+    ensures match res
+      case Success(frameWithGhostSeq) => ( // Decrypting the frame encoded in the stream is the returned ghost frame
+        && var decryptedFrame := frameWithGhostSeq.frame;
+           var ciphertext := frameWithGhostSeq.ciphertext;
+           var final := decryptedFrame.FinalFrame?;
+           decryptedFrame.Valid()
+        && old(rd.reader.pos) < rd.reader.pos <= |rd.reader.data|
+        && AESEncryption.CiphertextGeneratedWithPlaintext(ciphertext, decryptedFrame.encContent)      
+        && var encryptedFrame := (if decryptedFrame.FinalFrame? then
+             FinalFrame(decryptedFrame.seqNum, decryptedFrame.iv, ciphertext, decryptedFrame.authTag)
+           else
+             RegularFrame(decryptedFrame.seqNum, decryptedFrame.iv, ciphertext, decryptedFrame.authTag)); 
+           rd.reader.data[old(rd.reader.pos)..rd.reader.pos] == FrameToSequence(encryptedFrame)   
+        && AESEncryption.CiphertextGeneratedWithPlaintext(encryptedFrame.encContent, decryptedFrame.encContent))
       case Failure(_) => true
   {
     var final := false;
-    var sequenceNumber :- rd.ReadUInt32();
+    var sequenceNumber :- rd.ReadUInt32(); 
+    ghost var frameSerialization := UInt32ToSeq(sequenceNumber);
+    assert rd.reader.data[old(rd.reader.pos)..rd.reader.pos] == frameSerialization;
+    
     if sequenceNumber == ENDFRAME_SEQUENCE_NUMBER {
       final := true;
       sequenceNumber :- rd.ReadUInt32();
+      frameSerialization := frameSerialization + UInt32ToSeq(sequenceNumber);
+      assert rd.reader.data[old(rd.reader.pos)..rd.reader.pos] == frameSerialization;
     }
+    
     if sequenceNumber != expectedSequenceNumber {
       return Failure("unexpected frame sequence number");
     }
 
     var iv :- rd.ReadBytes(algorithmSuiteID.IVLength());
+    frameSerialization := frameSerialization + iv;
+    assert rd.reader.data[old(rd.reader.pos)..rd.reader.pos] == frameSerialization;
 
     var len := frameLength as uint32;
     if final {
       len :- rd.ReadUInt32();
+      if len > frameLength as uint32 {
+        return Failure("Final frame too long");
+      }
+      frameSerialization := frameSerialization + UInt32ToSeq(len);
     }
 
-    var aad := BodyAAD(messageID, if final then FinalFrame else RegularFrame, sequenceNumber, len as uint64);
+    var aad := BodyAAD(messageID, if final then AADFinalFrame else AADRegularFrame, sequenceNumber, len as uint64);
 
     var ciphertext :- rd.ReadBytes(len as nat);
+    frameSerialization := frameSerialization + ciphertext;
+    assert rd.reader.data[old(rd.reader.pos)..rd.reader.pos] == frameSerialization;
+    
     var authTag :- rd.ReadBytes(algorithmSuiteID.TagLength());
-    var plaintext :- Decrypt(ciphertext, authTag, algorithmSuiteID, iv, key, aad);
+    frameSerialization := frameSerialization + authTag;
+    assert rd.reader.data[old(rd.reader.pos)..rd.reader.pos] == frameSerialization;
 
-    return Success((plaintext, final));
+    var plaintext :- Decrypt(ciphertext, authTag, algorithmSuiteID, iv, key, aad);
+    assert AESEncryption.CiphertextGeneratedWithPlaintext(ciphertext, plaintext);
+    assert rd.reader.data[old(rd.reader.pos)..rd.reader.pos] == frameSerialization;
+
+    var frame := if final then
+        FinalFrame(sequenceNumber, iv, plaintext, authTag)
+      else 
+        RegularFrame(sequenceNumber, iv, plaintext, authTag);
+
+    ghost var encryptedFrame := if final then
+        FinalFrame(sequenceNumber, iv, ciphertext, authTag)
+      else 
+        RegularFrame(sequenceNumber, iv, ciphertext, authTag);    
+
+    // Feed dafny facts about the content of the stream
+    // Show dafny that the serialized frame is frameSerialization
+    assert frameSerialization == FrameToSequence(encryptedFrame);
+
+    // Prove read content of stream is frameSerialization 
+    assert !final ==> frameSerialization[..4] == rd.reader.data[old(rd.reader.pos)..][..4];
+    assert !final ==> frameSerialization[4..][..algorithmSuiteID.IVLength()] == rd.reader.data[old(rd.reader.pos)..][4..][..algorithmSuiteID.IVLength()];
+    assert !final ==> frameSerialization[4 + algorithmSuiteID.IVLength()..][..frameLength] == rd.reader.data[old(rd.reader.pos)..][4 + algorithmSuiteID.IVLength()..][..frameLength];
+    assert !final ==> frameSerialization[4 + frameLength + algorithmSuiteID.IVLength()..] == rd.reader.data[old(rd.reader.pos)..][4 + frameLength + algorithmSuiteID.IVLength()..][..algorithmSuiteID.TagLength()];
+
+    // Prove equivalence frameSerialization and content read on the stream
+    assert rd.reader.data[old(rd.reader.pos)..rd.reader.pos] == frameSerialization;
+
+    assert old(rd.reader.pos) < rd.reader.pos <= |rd.reader.data|;     
+
+    return Success(FrameWithGhostSeq(frame,ciphertext));
   }
 
   method BodyAAD(messageID: seq<uint8>, bc: BodyAADContent, sequenceNumber: uint32, length: uint64) returns (aad: seq<uint8>) {
@@ -187,6 +517,8 @@ module MessageBody {
     requires |iv| == algorithmSuiteID.IVLength()
     requires |key| == algorithmSuiteID.KeyLength()
     requires |authTag| == algorithmSuiteID.TagLength()
+    ensures res.Success? ==> AESEncryption.CiphertextGeneratedWithPlaintext(ciphertext, res.value)
+    ensures res.Success? ==> |ciphertext| == |res.value|
   {
     var encAlg := algorithmSuiteID.EncryptionSuite();
     res := AESEncryption.AESDecrypt(encAlg, key, ciphertext, authTag, iv, aad);
@@ -203,7 +535,7 @@ module MessageBody {
     var ciphertext :- rd.ReadBytes(contentLength as nat);
     var authTag :- rd.ReadBytes(algorithmSuiteID.TagLength());
 
-    var aad := BodyAAD(messageID, SingleBlock, NONFRAMED_SEQUENCE_NUMBER, contentLength);
+    var aad := BodyAAD(messageID, AADSingleBlock, NONFRAMED_SEQUENCE_NUMBER, contentLength);
 
     var plaintext :- Decrypt(ciphertext, authTag, algorithmSuiteID, iv, key, aad);
     return Success(plaintext);
